src/PrimitiveDecoder/BooleanVSTSpecEncoder.v
@@ -1,4 +1,3 @@
-(* VST specification of as *)
 Require Import Core.Core VstLib Lib BooleanExecSpec ErrorWithWriter.
 Require Import VST.floyd.proofauto Psatz.
 Require Import Clight.BOOLEAN.
@@ -67,10 +66,19 @@ Definition bool_der_encode_spec : ident * funspec :=
 
 Definition Gprog1 := ltac:(with_library prog [bool_der_encode_spec]).
 
-Theorem bool_der_encode : semax_body Vprog Gprog1 f_BOOLEAN_encode_der
-                                     bool_der_encode_spec.
-Admitted.
+Require Import StructNormalizer.
 
+Definition normalize_function f :=
+  mkfunction (fn_return f) (fn_callconv f) (fn_params f) (fn_vars f) (fn_temps f)
+             (struct_normalize (fn_body f) composites).
+
+Eval simpl in struct_normalize (fn_body f_BOOLEAN_encode_der) composites.
+
+
+Theorem bool_der_encode : semax_body Vprog Gprog1 (normalize_function f_BOOLEAN_encode_der)
+                                     bool_der_encode_spec.
+  start_function.
+Admitted.
 End Boolean_der_encode_primitive.
 
 
