src/Core/Core.v
@@ -1,4 +1,5 @@
 From Coq Require Export ZArith Psatz List String Sorting.Permutation.
+Export ListNotations.
 
 From compcert Require Export Coqlib Integers Floats AST Ctypes Cop Clight Clightdefs.
 From compcert Require Export Maps Values Events Memory.
