src/Core/StructNormalizer.v
@@ -1,0 +1,54 @@
+Require Import Core.Core.
+Import ListNotations.
+
+Fixpoint find_struct_fields (id : ident) (c : list composite_definition) :=
+  match c with
+  | [] => []
+  | h :: tl => match h with
+             | Composite id' _ ls _ => if (id =? id')%positive
+                                      then ls
+                                      else find_struct_fields id tl
+             end
+  end.
+
+Fixpoint ls_to_seq (ls : list statement) :=
+  match ls with
+  | [] => Sskip
+  | [h] => h
+  | h1 :: h2 :: tl => Ssequence h1 (Ssequence h2 (ls_to_seq tl))
+  end.
+
+Fixpoint copy_by_fields (p : positive) (id1 id2 : ident) (ty : type) (ls : members) :=
+  match ls with
+  | [] => []
+  | h :: tl => let f := fst h in
+             let t := snd h in
+             let s := Ssequence
+                        (Sset p (Efield (Evar id2 ty) f t))
+                        (Sassign  (Efield (Ederef (Etempvar id1 (tptr ty)) ty) f t) (Etempvar p t))
+             in
+             s :: copy_by_fields (p + 1)%positive id1 id2 ty tl
+  end.
+
+Fixpoint struct_normalize (s : statement) (c : list composite_definition) :=
+  match s with
+  | Ssequence s1 s2 => Ssequence (struct_normalize s1 c) (struct_normalize s2 c)
+  | Sloop s1 s2 => Sloop (struct_normalize s1 c) (struct_normalize s2 c)
+  | Sifthenelse e s1 s2 => Sifthenelse e (struct_normalize s1 c) (struct_normalize s2 c)
+  | Sswitch e ls => Sswitch e ((fix switch_normalize ls :=
+                                 match ls with
+                                 | LSnil => LSnil
+                                 | LScons z s ls' => LScons z (struct_normalize s c) (switch_normalize ls')
+                                 end) ls)
+  | Slabel l s => Slabel l (struct_normalize s c)
+  | Sassign (Evar id1 ty1) (Evar id2 ty2)
+  | Sassign (Etempvar id1 ty1) (Evar id2 ty2)
+  | Sassign (Ederef (Evar id1 ty1) _) (Evar id2 ty2)
+  | Sassign (Ederef (Etempvar id1 ty1) _) (Evar id2 ty2) =>
+    match ty2 with
+      | Tstruct _struct _ => let ls := find_struct_fields _struct c in 
+                            ls_to_seq (copy_by_fields 900%positive id1 id2 (Tstruct _struct noattr) ls)
+      | _ => s
+    end
+  | s => s 
+  end.
